\research{Basic Numeracy \& Algebra Worksheet 1}{02-10-22}{Worksheet}

1. Calculate:
\begin{align*}
    \frac{18}{6}\times 3 - 18 + 2 \times (-4) =&\\
    =& \frac{18}{6} \times 3 - 18 - 8 \\
    =& 3\times 3 - 18 - 8\\
    =& 9 - 18-8\\
    =&-9-8\\
    =&17
\end{align*}

2. Calculate:
\begin{align*}
    \frac{12}{6} + \frac{12}{-4} + (-2)\times (-1) =&\\
    =& \frac{12}{6} + \frac{12}{-4} + 2\\
    =& 2-3+2\\
    =& 1
\end{align*}

3. Calculate:
\begin{align*}
    (-3)\times(-1)-2-6+8 =&\\
    =& 3--4 + 8\\
    =& 3+4 + 8\\
    =& 15
\end{align*}

4. Calculate:
\begin{align*}
    (3^2\times 2 -2) \div 2^3 =&\\
    =& (9 \times 2 - 2) \div 2^3\\
    =& (18-2) \div 2^3\\
    =& (16) \div 2^3\\
    =& 16 \div 8\\
    =& 2
\end{align*}

5. Solve $\displaystyle 2x-8=3x-7$ for $x$.
\begin{align*}
    2x-8&=3x-7\\
    2x-1&=3x\\
    -1 &= 1x
\end{align*}

6. Solve $\displaystyle 4x-8 = 2(x+3)+10$ for x.
\begin{align*}
    4x-8 &= 2x+6+10\\
    4x-8 &= 2x+16\\
    4x &= 2x+24\\
    2x &= 24\\
    x &= 12
\end{align*}

7. Evaluate the expression $\displaystyle \frac{5}{3} - \frac{1}{3}\times \frac{9}{2}$ and write in its simplest form.
\begin{align*}
    \frac{5}{3} - \frac{1}{3}\times \frac{9}{2} &=\\
    &= \frac{5}{3} - \frac{9}{6}\\
    &= \frac{30}{18} - \frac{27}{18}\\
    &= \frac{3}{18}\\
    &= \frac{1}{6}
\end{align*}

8. Evaluate the expression $\displaystyle \frac{7}{2}-\frac{1}{4}+\frac{6}{8}$ and write it in its simplest form.
\begin{align*}
    \frac{7}{2}-\frac{1}{4}+\frac{6}{8} &=\\
    &= \left(\frac{7}{2} - \frac{1}{4}\right) + \frac{6}{8}\\
    &= \left(\frac{28}{8} - \frac{2}{8}\right) + \frac{6}{8}\\
    &= \left(\frac{28}{8}\right) + \frac{6}{8}\\
    &= \frac{32}{8}\\
    &= \frac{16}{4}\\
    &= \frac{4}{1}
\end{align*}

9. Simplify.
\begin{enumerate}
    \item[(i)] $3(-7y)$\\
    =$-21y$
    \item[(ii)] $(2y)(y^2)$\\
    =$3y^3$
    \item[(iii)] $3y^2(-2y)$\\
    =$6y^3$
    \item[(iv)] $(-2y)(-2y)$\\
    =$-4y^2$
\end{enumerate}

10. Expand the following expression
\begin{align*}
    2x(4x-\frac{1}{2})-4x(5-\frac{x}{2}) &=\\
    &= ...
\end{align*}

11. Expand the following expression
\begin{align*}
    6(4x+\frac{3}{2}) - 4x(5+\frac{x}{2} + x^2) &=\\
    &= ...
\end{align*}

12. Expand the following expression
\begin{align*}
    (x+3)(2x-6)+2 &=\\
    &= (2x^2-6x + 6x -18) + 2\\
    &= 2x-16
\end{align*}

13. Expand and fully simplify the following expression
\begin{align*}
    (2y-3)^2 &=\\
    &= (2y-3)(2y-3)\\
    &= 4y^2 - 6y - 6y +9\\
    &= 4y^2 -12y + 9
\end{align*}

14. Simplify the following expression.
\begin{align*}
    3x(x-y^2)+3(x^2+1)-7x^2y &=\\
    &= 3x^2 - 3xy^2 + 3x^2 + 3 - 7x^y\\
    &= 6x^2 - 3xy^2 + 3 - 7x^2y
\end{align*}