\lecture{Boolean Algebra Simplification II}{14-11-22}{16:00}{Farzad}{RB LT1}
NEW: Drop-in's this week are there for support. They are timetabled as Drop-Ins therefore not compulsory.

NB: From here-on, the $\overline{X}$ will be changing to $X'$ as I now know that this is the format which we will \textit{have} to use in the exam.

\section*{DeMorgan's Theorem}
\subsection*{Theorem 1}
\[(A \cdot B)' = A' + B'\]
\subsection*{Theorem 2}
\[(A+B)' = A' \cdot B'\]

\subsection*{Multi-Part DeMorgan's}
\begin{example}{Simplify $(A \cdot B + C)'$}
\begin{align*}
    (A \cdot B + C)' &= (A \cdot B)' \cdot C' && \mathrm{Apply\ DeMorgan's\ to\ OR}\\
    &= (A' + B') \cdot C' && \mathrm{Apply\ DeMorgan's\ to\ bracket}\\
    &= A' \cdot C' + B' \cdot C' && \mathrm{Expand\ bracket}
\end{align*}
\end{example}

\section*{How To Simplify}
\begin{enumerate}
    \item Apply De-Morgan's Theorem where possible. This will result in as single negated terms rather than bracketed negated terms
    \item Remove brackets where possible by applying distributive laws
    \item \label{ba-simp-rl} Apply rules \& laws to simplify
    \item \label{ba-simp-fact} Factorise the expression
    \item Iterate through steps \ref{ba-simp-rl} and \ref{ba-simp-fact} until the expression is simplified.
\end{enumerate}

\section*{Examples}
\subsection*{Example 1: Simplify}
\begin{align*}
A \cdot B \cdot C' + B \cdot C' + B' \cdot A &=\\ 
&= B \cdot C' \cdot (A + 1) + B' \cdot A\\
&= B \cdot C' \cdot 1 + B' \cdot A\\
&= B \cdot C' + B' \cdot A
\end{align*}
\subsection*{Example 2: Simplify}
\begin{align*}
A \cdot B + A \cdot (B+C) + B \cdot (B + C) &= \\
&= A\cdot B + A\cdot B + A\cdot C + B \cdot B + B \cdot C\\
&= A \cdot B + A \cdot C + B + B \cdot C \\
&= A \cdot B + A \cdot C + B (1 + C)\\
&= A \cdot B + A \cdot C + B\\
&= B + A\cdot C
\end{align*}
\subsection*{Example 3: Simplify}
\begin{align*}
\left([(B \cdot D + C)\cdot (A \cdot B')] + (B' \cdot A')\right) \cdot C &= \\
&= ([(B \cdot D + C)A\cdot B']+ A' \cdot B')\cdot C\\
&= [(A\cdot B' \cdot B \cdot D + A \cdot B' \cdot C) + A' \cdot B']\cdot C\\
&= A \cdot B \cdot B' \cdot C \cdot D + A \cdot B' \cdot C \cdot C + A' \cdot B' \cdot C\\
&= A \cdot B' \cdot C + A' \cdot B' \cdot C\\
&= B' \cdot C\cdot (A+A')\\
&= B' \cdot C \cdot (1)\\
&= B' \cdot C
\end{align*}
\subsection*{Example 4: Simplify}
\begin{align*}
A \cdot B' + A \cdot (B+C)' +B\cdot (B+C)' &= \\
&= A\cdot B' + A\cdot B' \cdot C' + B \cdot B' \cdot C'\\
&= A \cdot B' \cdot (1 + C')\\
&= A \cdot B' \cdot 1\\
&= A \cdot B'
\end{align*}